Update simplereplicaset controller spec

src/verification/simplereplicaset.v
@@ -7,22 +7,38 @@ Context `{!mapG Σ KKey.t (gset KKey.t)}.
 Context `{!auth_setG Σ KKey.t}.
 Context `{hG: !heapGS Σ} {go_ctx: GoContext}.
 
-Lemma wp_syncReplicaSet (namespace name: go_string) γ_state γ_children γ_fresh_keys rs_key rs s (n: w32):
+Definition active_pod (pod: v1.Pod.t) : bool :=
+  true.
+
+Definition active_child_count (child_pods: gmap KKey.t v1.Pod.t) : nat :=
+  length (filter (λ kv, active_pod (snd kv)) (map_to_list child_pods)).
+
+Lemma wp_syncReplicaSet namespace name
+  γ_state γ_children γ_fresh_keys rs_key rs child_keys child_pods (n: w32):
   {{{ is_pkg_init simplereplicaset ∗
       is_kubernetes_state γ_state γ_children γ_fresh_keys ∗
       ⌜ rs_key = mk_replicaset_key namespace name ⌝ ∗
       rs_key [[ γ_state ]]↦ KObject.ReplicaSet rs ∗
-      rs_key [[ γ_children ]]↦ s ∗
+      ([∗ map] key ↦ v ∈ child_pods,
+        key [[ γ_state ]]↦ KObject.Pod v ∗
+        ⌜ key ∈ child_keys ⌝) ∗
+      rs_key [[ γ_children ]]↦ child_keys ∗
+      ⌜ size child_pods = size child_keys ⌝ ∗
       rs.(v1.ReplicaSet.Spec').(v1.ReplicaSetSpec.Replicas') ↦ n
   }}}
   @! simplereplicaset.syncReplicaSet #namespace #name
-  {{{ (err : error.t) s', RET #err;
-      rs_key [[ γ_children ]]↦ s' ∗
+  {{{ (err : error.t) child_keys' child_pods', RET #err;
+      rs_key [[ γ_state ]]↦ KObject.ReplicaSet rs ∗
+      ([∗ map] key ↦ v ∈ child_pods',
+        key [[ γ_state ]]↦ KObject.Pod v ∗
+        ⌜ key ∈ child_keys' ⌝) ∗
+      rs_key [[ γ_children ]]↦ child_keys' ∗
+      ⌜ size child_pods' = size child_keys' ⌝ ∗
       if decide (err = interface.nil) then
-        ⌜ size s' = sint.nat n ⌝
+        ⌜ size child_keys' = sint.nat n ⌝
       else
-        ⌜ Z.abs (Z.of_nat (size s') - sint.Z n) <
-          Z.abs (Z.of_nat (size s) - sint.Z n) ⌝
+        ⌜ Z.abs (Z.of_nat (active_child_count child_pods) - sint.Z n) <
+          Z.abs (Z.of_nat (active_child_count child_pods') - sint.Z n) ⌝
   }}}.
 Proof. Admitted.
 
